Use insertion sort over mergesort

theories/BWT/Sorting/Key.v
@@ -1,23 +1,53 @@
 Require Import Coq.Lists.List.
 
 Require Import BWT.Sorting.Ord.
-Require Import BWT.Sorting.Mergesort.
+Require Import BWT.Sorting.InsertionSort.
 Require Import BWT.Sorting.Lexicographic.
 
 Section KeyOrd.
-  Context {K : Type} `{O: Ord K}.
+  Context {A K : Type} `{O: Ord K}.
 
-  Definition keyOrd {A : Type} (key : A -> K) : Ord A.
+  Variable key : A -> K.
+
+  Definition keyOrd : Ord A.
   Proof.
     apply Build_Ord with (le := fun x y => le (key x) (key y));
       intros; eauto using le_trans, le_total, le_dec.
   Defined.
+
+  Remark key_le_dec : forall x y,
+      @le_dec A keyOrd x y = @le_dec K O (key x) (key y).
+  Proof. reflexivity. Qed.
+
+  Section Inv.
+    Variable f : A -> A.
+    Hypothesis HF : forall x, key (f x) = key x.
+
+    Lemma key_insert_inv : forall x l,
+       @insert A keyOrd (f x) (map f l) = map f (@insert A keyOrd x l).
+    Proof.
+      induction l; [reflexivity|].
+      simpl. rewrite !HF.
+      destruct (le_dec (key x) (key a)).
+      - reflexivity.
+      - simpl; f_equal.
+        apply IHl.
+    Qed.
+
+    Theorem key_sort_inv : forall l,
+        @sort A keyOrd (map f l) = map f (@sort A keyOrd l).
+    Proof.
+      induction l; [reflexivity|].
+      simpl. rewrite <- key_insert_inv, IHl.
+      reflexivity.
+    Qed.
+  End Inv.
 End KeyOrd.
 
 Section HdSort.
   Context {A : Type} `{O: Ord A}.
 
   Program Definition hdsort : list (list A) -> list (list A)
-    := @mergesort _ (keyOrd (firstn 1)).
+    := @sort _ (keyOrd (firstn 1)).
 
 End HdSort.
