theories/BWT/Sorting/InsertionSort.v
@@ -1,0 +1,69 @@
+Require Import Coq.Lists.List.
+Require Import Coq.Sorting.Permutation.
+
+Require Import BWT.Sorting.Ord.
+Require Import BWT.Sorting.Sorted.
+
+Section InsertionSort.
+  Context {A : Type} {O : Ord A}.
+
+  Fixpoint insert (x : A) (l : list A) :=
+    match l with
+    | nil => x :: nil
+    | h::t => if le_dec x h then x :: h :: t else h :: insert x t
+    end.
+
+  Fixpoint sort (l: list A) : list A :=
+    match l with
+    | nil => nil
+    | h::t => insert h (sort t)
+    end.
+
+  Lemma insert_perm: forall x l, Permutation (x::l) (insert x l).
+  Proof.
+    intros. revert x. induction l as [ | hd tl IH]; intros x.
+    - simpl. apply Permutation_refl.
+    - simpl. destruct (le_dec x  hd).
+      + apply Permutation_refl.
+      + rewrite perm_swap. apply Permutation_cons.
+        reflexivity.
+        apply IH.
+  Qed.
+
+  Theorem sort_perm: forall l, Permutation l (sort l).
+  Proof.
+    induction l as [ | hd tl IH].
+    - simpl. apply Permutation_refl.
+    - simpl. apply perm_skip with (x := hd) in IH.
+      eapply perm_trans.
+      + apply IH.
+      + apply insert_perm.
+  Qed.
+
+  Lemma insert_sorted:
+    forall a l, Sorted l -> Sorted (insert a l).
+  Proof.
+    intros a l Sl; revert a.
+    induction Sl as [ | hd tl HIn HS IH]; intros a; [apply Sorted_1|].
+    simpl; destruct (le_dec a hd).
+    - apply Sorted_cons.
+      intros x HIn'; simpl in HIn'.
+      destruct HIn'; [subst; auto|].
+      eapply le_trans. apply l. apply HIn; auto.
+      constructor. apply HIn. apply HS.
+    - apply Sorted_cons.
+      intros x HIn'.
+      apply Permutation_in with (l' := a::tl) in HIn';
+        [|auto using insert_perm, Permutation_sym].
+      destruct HIn'; [subst; apply le_not; auto|].
+      apply HIn; auto.
+      apply IH.
+  Qed.
+
+  Theorem sort_sorted: forall l, Sorted (sort l).
+  Proof.
+    induction l as [ | hd tl IH].
+    - simpl. apply Sorted_nil.
+    - simpl. apply insert_sorted. apply IH.
+  Qed.
+End InsertionSort.
